theories/examples/adder.v
@@ -350,14 +350,8 @@ Section adder.
     (* Step 1: Use the spec for g *)
     iApply (adder_g_spec with "[- $HPC $Hr0 $Hr1 $Hr2 $Hr3 $Hact $Hprog_g]"); auto.
     (* Step 2: Use the validity of w0 and the FTLR *)
-    iPoseProof (jmp_or_fail_spec _ (λ _, True)%I with "Hw0") as "Hcont".
-    destruct (decide (isCorrectPC (updatePcPerm w0))); cycle 1.
-    { (* the jump might fail: that's OK. *)
-      iNext. iIntros "(? & ? & ? & ? & ? & ?)".
-      iApply "Hcont". iFrame. }
-    (* otherwise, we get that the continuation satisfies the expression relation *)
-    iDestruct "Hcont" as (p b e a ->) "#Ew0". iNext.
-    iIntros "(HPC & Hprog_g & Hr0 & Hr1 & Hr2 & Hr3 & Hact)".
+    iPoseProof (jmp_to_unknown with "Hw0") as "Hcont_g".
+    iNext. iIntros "(HPC & Hprog_g & Hr0 & Hr1 & Hr2 & Hr3 & Hact)".
 
     (* Step 3: Prove that the closure is valid, by using the spec of [f] *)
     (* Put the code of [f] and the activation record in invariants *)
@@ -366,9 +360,9 @@ Section adder.
 
     iAssert (interp (inr (E, act_start, act_end, act_start))) with "[Iprog_f Iact]"
       as "Hclosure".
-    { iClear "Ew0 Hw0". rewrite /interp /= fixpoint_interp1_eq /=.
+    { iClear "Hw0". rewrite /interp /= fixpoint_interp1_eq /=.
       iIntros (rmap'). iNext. iModIntro. iIntros "([Hrmap' #HrV] & Hregs & HnaI)".
-      iDestruct "Hrmap'" as %Hrmap'. iSplit; eauto. rewrite /interp_conf.
+      iDestruct "Hrmap'" as %Hrmap'. rewrite /interp_conf.
       (* extract registers relevant for f from the map *)
       iDestruct (big_sepM_delete _ _ PC with "Hregs") as "[HPC Hregs]".
       by rewrite lookup_insert.
@@ -405,13 +399,9 @@ Section adder.
         (* This involves a lot of bureaucratic shuffling of the register resources *)
         unshelve iPoseProof ("HrV" $! r_t0 _) as "Hr0V";[done|].
         rewrite /RegLocate Hrv0.
-        pose (λ v, ⌜v = HaltedV⌝ → ∃ r, full_map r ∧ registers_mapsto r ∗ na_own logrel_nais ⊤)%I as φ.
-        iPoseProof (jmp_or_fail_spec _ φ with "Hr0V") as "Hcont".
-        destruct (decide (isCorrectPC (updatePcPerm rv0))); cycle 1.
-        { iNext. iIntros "H". iApply "Hcont". iDestruct "H" as (? ?) "(? & ?)". iFrame.
-          rewrite /φ /=. iIntros (?). congruence. }
-        iDestruct "Hcont" as (p' b' e' a' ->) "Hcont". iNext.
-        iIntros "HH". iDestruct "HH" as (k' n') "(HPC & Hprog_f & Hr0 & Hr1 & Hr2 & Hr3 & Hrenv)".
+        iPoseProof (jmp_to_unknown with "Hr0V") as "Hcont".
+        iNext. iIntros "H".
+        iDestruct "H" as (k' n') "(HPC & Hprog_f & Hr0 & Hr1 & Hr2 & Hr3 & Hrenv)".
         iDestruct ("Hprog_f_close" with "[$HnaI $Hprog_f]") as ">HnaI". (* close *)
         (* Put the registers back in the map *)
         iDestruct (big_sepM_insert with "[$Hregs $Hr0]") as "Hregs".
@@ -429,45 +419,18 @@ Section adder.
         iDestruct (big_sepM_insert with "[$Hregs $Hrenv]") as "Hregs".
         by repeat (rewrite lookup_delete_ne //;[]); rewrite lookup_delete //.
         repeat (rewrite -delete_insert_ne //;[]). rewrite insert_delete.
-        iDestruct (big_sepM_insert with "[$Hregs $HPC]") as "Hregs".
-        rewrite !lookup_insert_ne // lookup_delete //.
         match goal with |- context [ ([∗ map] _↦_ ∈ ?r, _)%I ] => set rmap'' := r end.
-        iAssert (full_map rmap'') as %Hrmap''_full.
-        { rewrite /full_map. iIntros (rr). iPureIntro. rewrite elem_of_gmap_dom /rmap''.
-          rewrite !dom_insert_L !dom_delete_L !dom_insert_L regmap_full_dom //.
-          rewrite !singleton_union_difference_L !all_registers_union_l.
-          pose proof (all_registers_s_correct rr) as HH. set_solver+ HH. }
-
-        iSpecialize ("Hcont" $! rmap'' with "[Hregs HnaI]").
-        { iFrame. iSplitR.
-          { rewrite /interp_reg /=. iSplit; auto. iIntros (r Hr).
-            specialize (Hrmap''_full r) as [rv Hrv]. rewrite /RegLocate Hrv.
-            unshelve iSpecialize ("HrV" $! r _); auto.
-            rewrite /rmap'' in Hrv. rewrite (fixpoint_interp1_eq rv).
-            destruct (decide (r = r_env)); subst.
-            { rewrite lookup_insert_ne // lookup_insert in Hrv. by simplify_eq. }
-            destruct (decide (r = r_t3)); subst.
-            { repeat (rewrite lookup_insert_ne // in Hrv;[]); rewrite lookup_insert // in Hrv.
-              by simplify_eq. }
-            destruct (decide (r = r_t2)); subst.
-            { repeat (rewrite lookup_insert_ne // in Hrv;[]); rewrite lookup_insert // in Hrv.
-              by simplify_eq. }
-            destruct (decide (r = r_t1)); subst.
-            { repeat (rewrite lookup_insert_ne // in Hrv;[]); rewrite lookup_insert // in Hrv.
-              by simplify_eq. }
-            destruct (decide (r = r_t0)); subst.
-            { repeat (rewrite lookup_insert_ne // in Hrv;[]); rewrite lookup_insert // in Hrv.
-              simplify_eq. rewrite !fixpoint_interp1_eq //. }
-            repeat (rewrite lookup_insert_ne // in Hrv;[]).
-            rewrite delete_insert_delete lookup_delete_ne // in Hrv.
-            rewrite Hrv !fixpoint_interp1_eq //. }
-          { rewrite /registers_mapsto /rmap'' insert_insert //. } }
-
-        iDestruct "Hcont" as "[_ Hcont]". rewrite /interp_conf.
-        iApply (wp_wand with "[-]"). iApply "Hcont". cbn. iIntros (v) "?". eauto.
-      }
-      { cbn. iIntros (?) "[H|%]"; iIntros (->). iApply "H"; eauto. congruence. }
-    }
+        iApply "Hcont"; cycle 1.
+        { iFrame. iApply (big_sepM_sep with "[$Hregs HrV]"). cbn beta.
+          repeat (iApply big_sepM_insert_2; first by rewrite /= !fixpoint_interp1_eq //).
+          rewrite delete_insert_delete.
+          iApply big_sepM_intuitionistically_forall. iModIntro.
+          iIntros (r' ? Hr'). eapply lookup_delete_Some in Hr' as [? Hr'].
+          unshelve iSpecialize ("HrV" $! r' _). done. by rewrite Hr'. }
+        { iPureIntro. rewrite !dom_insert_L dom_delete_L dom_insert_L.
+          rewrite regmap_full_dom //. set_solver+. } }
+      { cbn beta. iIntros (?) "H". iIntros (->). iDestruct "H" as "[H|%]". 2: congruence.
+        iApply "H". done. } }
 
     (* Step 4: use the fact that the continuation is in the expression relation *)
     (* put the registers back in the map *)
@@ -483,28 +446,10 @@ Section adder.
     iDestruct (big_sepM_insert with "[$Hregs $Hr0]") as "Hregs".
     { rewrite !lookup_insert_ne //. apply elem_of_gmap_dom_none. set_solver+ Hrmap_dom. }
     { eauto. }
-    match goal with |- context [ ([∗ map] _↦_ ∈ ?r, _)%I ] => set rmap' := r end.
-    iDestruct (big_sepM_sep with "Hregs") as "[Hregs HregsV]".
-    iDestruct (big_sepM_insert with "[$Hregs $HPC]") as "Hregs".
-    { rewrite !lookup_insert_ne //. apply elem_of_gmap_dom_none. set_solver+ Hrmap_dom. }
-    set rmap'' := <[_:=_]> rmap'.
-    iAssert (full_map rmap'') as %Hrmap''_full.
-    { rewrite /full_map. iIntros (rr). iPureIntro. rewrite elem_of_gmap_dom /rmap'' /rmap'.
-      rewrite !dom_insert_L Hrmap_dom.
-      rewrite !singleton_union_difference_L !all_registers_union_l.
-      pose proof (all_registers_s_correct rr) as H. set_solver+ H. }
 
-    iSpecialize ("Ew0" $! rmap'' with "[Hregs HregsV HnaI]").
-    { iFrame. iSplitR "Hregs"; cycle 1.
-      { rewrite /registers_mapsto /rmap'' insert_insert. eauto. }
-      rewrite /interp_reg /=. iSplit; eauto. iIntros (r Hr).
-      destruct (Hrmap''_full r) as [rv Hrv].
-      iDestruct (big_sepM_lookup _ _ r with "HregsV") as "Hr"; eauto.
-      rewrite /rmap'' /RegLocate (lookup_insert_ne _ PC) // in Hrv |- *.
-      rewrite Hrv //. }
-
-    iDestruct "Ew0" as "[_ Hcont]". iApply (wp_wand with "[-]"). iApply "Hcont".
-    eauto.
+    iApply "Hcont_g"; cycle 1. by iFrame.
+    iPureIntro. rewrite !dom_insert_L Hrmap_dom.
+    rewrite !singleton_union_difference_L !all_registers_union_l. set_solver+.
   Qed.
 
 End adder.
