theories/ftlr/interp_weakening.v
@@ -50,7 +50,7 @@ Section fundamental.
     intros HpnotE Hb He Hp. iIntros "#IH #HA".
     destruct (decide (b' <= e')%a).
     2: { rewrite !fixpoint_interp1_eq. destruct p'; try done; try (by iClear "HA"; rewrite /= !region_addrs_empty;[|solve_addr]).
-         iIntros (r). iNext. iModIntro. iIntros "([Hfull Hreg] & Hregs & Hna)". iSplit;auto.
+         iIntros (r). iNext. iModIntro. iIntros "([Hfull Hreg] & Hregs & Hna)".
          iApply ("IH" with "Hfull Hreg Hregs Hna"); auto. iModIntro.
          iClear "HA". by rewrite !fixpoint_interp1_eq /= !region_addrs_empty;[|solve_addr]. 
     }  
@@ -74,7 +74,7 @@ Section fundamental.
       rewrite !big_sepL_app; iDestruct "HA" as "[A1 [A2 A3]]";iFrame "#".
       iApply (big_sepL_mono with "A2").
       iIntros (k y Hsome) "H". iDestruct "H" as (P) "(H1 & H2 & H3)". iExists P. iFrame.
-    - rewrite !fixpoint_interp1_eq. iIntros (r). iNext. iModIntro. iIntros "([Hfull Hreg] & Hregs & Hna)". iSplit;auto.
+    - rewrite !fixpoint_interp1_eq. iIntros (r). iNext. iModIntro. iIntros "([Hfull Hreg] & Hregs & Hna)".
       iApply ("IH" with "Hfull Hreg Hregs Hna"); auto. iModIntro.
       destruct p; inversion Hp; try contradiction.
       + rewrite /= (isWithin_region_addrs_decomposition b' e' b e); [|solve_addr].
